ironfleet/src/Dafny/Distributed/Protocol/RSL/FailureProof/Common/assumptions.i.dfy
@@ -1,0 +1,59 @@
+include "../TimestampedRslSystem.i.dfy"
+include "../../CommonProof/Constants.i.dfy"
+
+module Common_Assumptions {
+import opened TimestampedRslSystem_i
+import opened CommonProof__Constants_i
+
+
+
+/*****************************************************************************************
+*                                     Assumptions                                        *
+*****************************************************************************************/
+
+
+predicate CommonAssumptions(ts:TimestampedRslState) {
+    && RslConsistency(ts)
+    && NoPacketDuplication(ts)
+    && NoExternalPackets(ts)
+    && NoExternalSteps(ts)
+    && BoundedQueueingAssumption(ts)
+    && |ts.t_replicas| > 2  // For failure to be meaningful
+    && ts.t_replicas[0].v.replica.proposer.constants.all.params.max_batch_size > 0
+    && ts.t_replicas[1].v.replica.proposer.constants.all.params.max_batch_size > 0
+    && ts.constants.params.max_batch_size == 1
+}
+
+predicate NoExternalPackets(ts:TimestampedRslState) {
+    forall pkt | pkt in ts.undeliveredPackets ::
+        && pkt in ts.t_environment.sentPackets
+        && pkt.src in ts.constants.config.replica_ids
+        && pkt.dst in ts.constants.config.replica_ids
+}
+
+predicate NoExternalSteps(ts:TimestampedRslState) {
+    !(exists eid, ios :: ts.t_environment.nextStep == LEnvStepHostIos(eid, ios, ExternalStep()))
+}
+
+// Bounded queueing assumption for simplified RSL
+predicate BoundedQueueingAssumption(ts:TimestampedRslState) 
+    requires RslConsistency(ts)
+{
+    forall idx, ios :: (
+        && 0 <= idx < |ts.constants.config.replica_ids|
+        && ts.t_environment.nextStep == LEnvStepHostIos(ts.constants.config.replica_ids[idx], ios, RslStep(ts.t_replicas[idx].v.nextActionIndex))
+        ==>
+        (forall io | io in ts.t_environment.nextStep.ios && io.LIoOpReceive? ::
+            // this means that max(replica.ts, msg.ts) <= msg.ts + MaxQueueTime
+            ts.t_replicas[idx].ts <= io.r.msg.ts + MaxQueueTime
+        )
+    )
+}
+
+predicate RslConsistency(ts:TimestampedRslState)
+{
+    ConstantsAllConsistentInv(UntimestampRslState(ts))
+        && WellFormedLConfiguration(ts.constants.config)
+}
+
+}
