ironfleet/src/Dafny/Distributed/Protocol/RSL/FailureProof/TopLevel/FailureProof.i.dfy
@@ -1,0 +1,86 @@
+include "../TimestampedRslSystem.i.dfy"
+include "../../CommonProof/Constants.i.dfy"
+
+include "../Failover/FailureDetection_toplevel.i.dfy"
+include "../Phase2_PostFail/Phase2Proof_toplevel.i.dfy"
+include "../Common/assumptions.i.dfy"
+
+
+module RslFailureProof_i {
+import opened TimestampedRslSystem_i
+import opened CommonProof__Constants_i
+import opened Common_Assumptions
+
+import FOStg_Def = FailureDetection_defns_i
+import P2Stg_Pf = Rs2Phase2Proof_PostFail_Top  
+import P2Stg_Def = RslPhase2Proof_PostFail_i
+
+/*****************************************************************************************
+*                                      Guarantees                                        *
+*****************************************************************************************/
+
+/* Main performance guarantee */
+predicate PerformanceGuarantee_Final(ts:TimestampedRslState) 
+    requires |ts.t_replicas| > 2
+    requires RslConsistency(ts)
+{
+    forall pkt | 
+        && pkt in ts.undeliveredPackets 
+        && P2Stg_Def.IsNewReplyPacket(ts, pkt)
+    :: TimeLe(pkt.msg.ts, P2Stg_Def.TimeBoundReplyFinal())
+}
+
+
+/*****************************************************************************************
+*                                     Assumptions                                        *
+*****************************************************************************************/
+
+/* Conjunction of all assumptions */
+predicate RslAssumption(ts:TimestampedRslState, opn:OperationNumber)
+{
+    && CommonAssumptions(ts)
+    && (InPhase2Stage(ts) ==> P2Stg_Def.RslAssumption(ts, opn))
+    && (InFailoverStage(ts) ==> FOStg_Def.RslAssumption(ts))
+}
+
+predicate RslAssumption2(ts:TimestampedRslState, ts':TimestampedRslState)
+{
+    (InFailoverStage(ts) && InFailoverStage(ts') ==> FOStg_Def.RslAssumption2(ts, ts'))
+}
+
+
+
+/*****************************************************************************************
+*                                     Invariants                                        *
+*****************************************************************************************/
+
+
+// // Main invariant 
+// predicate RslPerfInvariant(ts:TimestampedRslState, opn:OperationNumber) 
+//     requires |ts.t_replicas| > 2
+// {
+//     && RslConsistency(ts)
+//     && AlwaysInvariant(ts, opn)
+//     && PerformanceGuarantee(ts, opn)
+//     && PacketsBallotInvariant(ts)
+//     && (|| Before_2a_Sent_Invariant(ts, opn)
+//         || Before_2b_Sent_Invariant(ts, opn)
+//         || After_2b_Sent_Invariant(ts, opn)
+//     )
+// }
+
+
+/*****************************************************************************************
+*                                  Misc Definitions                                      *
+*****************************************************************************************/
+
+
+
+
+predicate InFailoverStage(ts:TimestampedRslState) 
+
+predicate InPhase1Stage(ts:TimestampedRslState) 
+
+predicate InPhase2Stage(ts:TimestampedRslState) 
+
+}
