ironfleet/src/Dafny/Distributed/Protocol/RSL/FailureProof/TopLevel/notes.md
@@ -1,0 +1,15 @@
+# Failure Detection
+
+## Assumptions
+
+* `RslConsistency(s)`
+* `BoundedQueueingAssumption(s)`
+* `NoStateTransfer(s)`: State-Request, State-Supply and Starting-Phase2 messages are never received.
+* `NoExternalSteps(s)`
+* `OneAndOnlyOneRequest(s)`: there is a ghost constant `req`, and the system contains only this request.
+
+* `ClockAssumption(s, s')`
+    * When a replica `r` reads the clock in `s` to obtain value `t`, it must be that `r.ts <= t <= r'.ts`.
+
+
+
